WIP: Make all Locmap accesses go through Locmap.get
To prepare for register pairs stored in Locmap.t instances, change its type
so that users must go through the Locmap.get function or the new @ notation
to access the value stored at a location.

backend/Allocproof.v
@@ -432,7 +432,7 @@ Definition sel_val (k: equation_kind) (v: val) : val :=
   is less defined than [ls l] (the value of [l] in the LTL code). *)
 
 Definition satisf (rs: regset) (ls: locset) (e: eqs) : Prop :=
-  forall q, EqSet.In q e -> Val.lessdef (sel_val (ekind q) rs#(ereg q)) (ls (eloc q)).
+  forall q, EqSet.In q e -> Val.lessdef (sel_val (ekind q) rs#(ereg q)) (ls @ (eloc q)).
 
 Lemma empty_eqs_satisf:
   forall rs ls, satisf rs ls empty_eqs.
@@ -458,7 +458,7 @@ Qed.
 
 Lemma add_equation_lessdef:
   forall rs ls q e,
-  satisf rs ls (add_equation q e) -> Val.lessdef (sel_val (ekind q) rs#(ereg q)) (ls (eloc q)).
+  satisf rs ls (add_equation q e) -> Val.lessdef (sel_val (ekind q) rs#(ereg q)) (ls @ (eloc q)).
 Proof.
   intros. apply H. unfold add_equation. simpl. apply EqSet.add_1. auto.
 Qed.
@@ -1074,9 +1074,9 @@ Lemma subst_loc_satisf:
   subst_loc dst src e = Some e' ->
   loc_type_compat env dst e = true ->
   wt_regset env rs ->
-  Val.has_type (ls src) (Loc.type dst) ->
+  Val.has_type (ls @ src) (Loc.type dst) ->
   satisf rs ls e' ->
-  satisf rs (Locmap.set dst (ls src) ls) e.
+  satisf rs (Locmap.set dst (ls @ src) ls) e.
 Proof.
   intros; red; intros.
   exploit in_subst_loc; eauto. intros [[A B] | [A B]].
@@ -1138,9 +1138,9 @@ Qed.
 Lemma subst_loc_part_satisf_lowlong:
   forall src dst rs ls e e',
   subst_loc_part (R dst) (R src) Low e = Some e' ->
-  Val.has_type (Val.loword (ls (R src))) (mreg_type dst) ->
+  Val.has_type (Val.loword (ls @ (R src))) (mreg_type dst) ->
   satisf rs ls e' ->
-  satisf rs (Locmap.set (R dst) (Val.loword (ls (R src))) ls) e.
+  satisf rs (Locmap.set (R dst) (Val.loword (ls @ (R src))) ls) e.
 Proof.
   intros; red; intros.
   exploit in_subst_loc_part; eauto. intros [[A [B C]] | [A B]].
@@ -1152,9 +1152,9 @@ Qed.
 Lemma subst_loc_part_satisf_highlong:
   forall src dst rs ls e e',
   subst_loc_part (R dst) (R src) High e = Some e' ->
-  Val.has_type (Val.hiword (ls (R src))) (mreg_type dst) ->
+  Val.has_type (Val.hiword (ls @ (R src))) (mreg_type dst) ->
   satisf rs ls e' ->
-  satisf rs (Locmap.set (R dst) (Val.hiword (ls (R src))) ls) e.
+  satisf rs (Locmap.set (R dst) (Val.hiword (ls @ (R src))) ls) e.
 Proof.
   intros; red; intros.
   exploit in_subst_loc_part; eauto. intros [[A [B C]] | [A B]].
@@ -1241,8 +1241,8 @@ Lemma subst_loc_pair_satisf_makelong:
   wt_regset env rs ->
   satisf rs ls e' ->
   Archi.ptr64 = false ->
-  Val.has_type (Val.longofwords (ls (R src1)) (ls (R src2))) (mreg_type dst) ->
-  satisf rs (Locmap.set (R dst) (Val.longofwords (ls (R src1)) (ls (R src2))) ls) e.
+  Val.has_type (Val.longofwords (ls @ (R src1)) (ls @ (R src2))) (mreg_type dst) ->
+  satisf rs (Locmap.set (R dst) (Val.longofwords (ls @ (R src1)) (ls @ (R src2))) ls) e.
 Proof.
   intros; red; intros.
   exploit in_subst_loc_pair; eauto. intros [[A [B [C D]]] | [A B]].
@@ -1271,7 +1271,7 @@ Qed.
 
 Lemma undef_regs_outside:
   forall ml ls l,
-  Loc.notin l (map R ml) -> undef_regs ml ls l = ls l.
+  Loc.notin l (map R ml) -> (undef_regs ml ls) @ l = ls @ l.
 Proof.
   induction ml; simpl; intros. auto.
   rewrite Locmap.gso. apply IHml. tauto. apply Loc.diff_sym. tauto.
@@ -1307,7 +1307,7 @@ Lemma subst_loc_undef_satisf:
   can_undef_except dst ml e = true ->
   wt_regset env rs ->
   satisf rs ls e' ->
-  satisf rs (Locmap.set dst (ls src) (undef_regs ml ls)) e.
+  satisf rs (Locmap.set dst (ls @ src) (undef_regs ml ls)) e.
 Proof.
   intros; red; intros.
   exploit in_subst_loc; eauto. intros [[A B] | [A B]].
@@ -1358,13 +1358,13 @@ Definition callee_save_loc (l: loc) :=
   end.
 
 Definition agree_callee_save (ls1 ls2: locset) : Prop :=
-  forall l, callee_save_loc l -> ls1 l = ls2 l.
+  forall l, callee_save_loc l -> ls1 @ l = ls2 @ l.
 
 Lemma return_regs_agree_callee_save:
   forall caller callee,
   agree_callee_save caller (return_regs caller callee).
 Proof.
-  intros; red; intros. unfold return_regs. red in H.
+  intros; red; intros. unfold Locmap.get, return_regs. red in H.
   destruct l.
   rewrite H; auto.
   destruct sl; auto || congruence.
@@ -1491,9 +1491,9 @@ Proof.
   red; intros. rewrite Regmap.gsspec. destruct (peq (ereg q) r1).
   exploit compat_left2_sound; eauto.
   intros [[A B] | [A B]]; rewrite A; rewrite B; simpl.
-  apply Val.lessdef_trans with (Val.hiword (Val.longofwords (ls l1) (ls l2))).
+  apply Val.lessdef_trans with (Val.hiword (Val.longofwords (ls @ l1) (ls @ l2))).
   apply Val.hiword_lessdef; auto. apply val_hiword_longofwords.
-  apply Val.lessdef_trans with (Val.loword (Val.longofwords (ls l1) (ls l2))).
+  apply Val.lessdef_trans with (Val.loword (Val.longofwords (ls @ l1) (ls @ l2))).
   apply Val.loword_lessdef; auto. apply val_loword_longofwords.
   eapply IHb; eauto.
 - (* error case *)
@@ -1510,8 +1510,8 @@ Proof.
   assert (A: forall l, loc_argument_acceptable l -> call_regs ls (parameter_of_argument l) = ls l).
   { destruct l as [r | [] ofs ty]; simpl; auto; contradiction. }
   exploit loc_arguments_acceptable; eauto. destruct x; simpl; intros.
-- auto.
-- destruct H0; f_equal; auto.
+- unfold Locmap.get. rewrite A; auto.
+- unfold Locmap.get. destruct H0; f_equal; rewrite A; auto.
 Qed.
 
 Lemma return_regs_arg_values:
@@ -1526,7 +1526,7 @@ Proof.
   apply Locmap.getpair_exten; intros.
   assert (In l (regs_of_rpairs (loc_arguments sg))) by (eapply in_regs_of_rpairs; eauto).
   exploit loc_arguments_acceptable_2; eauto. exploit H; eauto.
-  destruct l; simpl; intros; try contradiction. rewrite H4; auto.
+  destruct l; simpl; intros; try contradiction. unfold Locmap.get, return_regs. rewrite H4; auto.
 Qed.
 
 Lemma find_function_tailcall:
@@ -1536,7 +1536,7 @@ Lemma find_function_tailcall:
 Proof.
   unfold ros_compatible_tailcall, find_function; intros.
   destruct ros as [r|id]; auto.
-  unfold return_regs. destruct (is_callee_save r). discriminate. auto.
+  unfold Locmap.get, return_regs. destruct (is_callee_save r). discriminate. auto.
 Qed.
 
 Lemma loadv_int64_split:
@@ -1572,15 +1572,15 @@ Lemma add_equations_builtin_arg_lessdef:
   add_equations_builtin_arg env arg arg' e = Some e' ->
   satisf rs ls e' ->
   wt_regset env rs ->
-  exists v', eval_builtin_arg ge ls sp m arg' v' /\ Val.lessdef v v'.
+  exists v', eval_builtin_arg ge (Locmap.read ls) sp m arg' v' /\ Val.lessdef v v'.
 Proof.
   induction 1; simpl; intros e e' arg' AE SAT WT; destruct arg'; MonadInv.
 - exploit add_equation_lessdef; eauto. simpl; intros.
-  exists (ls x0); auto with barg.
+  exists (ls @ x0); econstructor; auto with barg; econstructor.
 - destruct arg'1; MonadInv. destruct arg'2; MonadInv.
   exploit add_equation_lessdef. eauto. simpl; intros LD1.
   exploit add_equation_lessdef. eapply add_equation_satisf. eauto. simpl; intros LD2.
-  exists (Val.longofwords (ls x0) (ls x1)); split; auto with barg.
+  exists (Val.longofwords (ls @ x0) (ls @ x1)); split; auto with barg. econstructor; econstructor.
   rewrite <- (val_longofwords_eq_2 rs#x); auto. apply Val.longofwords_lessdef; auto.
   rewrite <- e0; apply WT.
 - econstructor; eauto with barg.
@@ -1618,14 +1618,15 @@ Lemma add_equations_builtin_args_lessdef:
   satisf rs ls e' ->
   wt_regset env rs ->
   Mem.extends m tm ->
-  exists vl', eval_builtin_args ge ls sp tm arg' vl' /\ Val.lessdef_list vl vl'.
+  exists vl', eval_builtin_args ge (Locmap.read ls) sp tm arg' vl' /\ Val.lessdef_list vl vl'.
 Proof.
   induction 1; simpl; intros; destruct arg'; MonadInv.
 - exists (@nil val); split; constructor.
 - exploit IHlist_forall2; eauto. intros (vl' & A & B).
   exploit add_equations_builtin_arg_lessdef; eauto.
   eapply add_equations_builtin_args_satisf; eauto. intros (v1' & C & D).
-  exploit (@eval_builtin_arg_lessdef _ ge ls ls); eauto. intros (v1'' & E & F).
+  exploit (@eval_builtin_arg_lessdef _ ge (Locmap.read ls) (Locmap.read ls)); eauto.
+  intros (v1'' & E & F).
   exists (v1'' :: vl'); split; constructor; auto. eapply Val.lessdef_trans; eauto.
 Qed.
 
@@ -1647,7 +1648,7 @@ Lemma add_equations_debug_args_eval:
   satisf rs ls e' ->
   wt_regset env rs ->
   Mem.extends m tm ->
-  exists vl', eval_builtin_args ge ls sp tm arg' vl'.
+  exists vl', eval_builtin_args ge (Locmap.read ls) sp tm arg' vl'.
 Proof.
   induction 1; simpl; intros; destruct arg'; MonadInv.
 - exists (@nil val); constructor.
@@ -1656,7 +1657,8 @@ Proof.
 + exploit IHlist_forall2; eauto. intros (vl' & B).
   exploit add_equations_builtin_arg_lessdef; eauto.
   eapply add_equations_debug_args_satisf; eauto. intros (v1' & C & D).
-  exploit (@eval_builtin_arg_lessdef _ ge ls ls); eauto. intros (v1'' & E & F).
+  exploit (@eval_builtin_arg_lessdef _ ge (Locmap.read ls) (Locmap.read ls)); eauto.
+  intros (v1'' & E & F).
   exists (v1'' :: vl'); constructor; auto.
 + eauto.
 Qed.
@@ -1674,7 +1676,7 @@ Lemma add_equations_builtin_eval:
   external_call ef ge vargs m1 t vres m2 ->
   satisf rs ls e1 /\
   exists vargs' vres' m2',
-     eval_builtin_args ge ls sp m1' args' vargs'
+     eval_builtin_args ge (Locmap.read ls) sp m1' args' vargs'
   /\ external_call ef ge vargs' m1' t vres' m2'
   /\ Val.lessdef vres vres'
   /\ Mem.extends m2 m2'.
@@ -1683,7 +1685,7 @@ Proof.
   assert (DEFAULT: add_equations_builtin_args env args args' e1 = Some e2 ->
     satisf rs ls e1 /\
     exists vargs' vres' m2',
-       eval_builtin_args ge ls sp m1' args' vargs'
+       eval_builtin_args ge (Locmap.read ls) sp m1' args' vargs'
     /\ external_call ef ge vargs' m1' t vres' m2'
     /\ Val.lessdef vres vres'
     /\ Mem.extends m2 m2').
@@ -1937,34 +1939,34 @@ Opaque destroyed_by_op.
 * (* stack->stack *)
   inv H0. simpl in H8. contradiction.
 + (* makelong *)
-  assert (HT: Val.has_type (Val.longofwords (ls (R src1)) (ls (R src2))) (mreg_type dst)).
+  assert (HT: Val.has_type (Val.longofwords (ls @ (R src1)) (ls @ (R src2))) (mreg_type dst)).
   {
     destruct H3; InvBooleans. simpl in H6.
     destruct (mreg_type dst) eqn:T; simpl; auto; inversion H6.
-    destruct (ls (R src1)), (ls (R src2)); simpl; auto.
-    destruct (ls (R src1)), (ls (R src2)); simpl; auto.
+    destruct (ls @ (R src1)), (ls @ (R src2)); simpl; auto.
+    destruct (ls @ (R src1)), (ls @ (R src2)); simpl; auto.
   }
   exploit IHmv; eauto. eapply subst_loc_pair_satisf_makelong; eauto.
   destruct H3; InvBooleans. split; eauto using wt_setreg.
   intros [ls' [A B]]. exists ls'; split; auto. eapply star_left; eauto.
   econstructor. simpl; eauto. reflexivity. traceEq.
 + (* lowlong *)
-  assert (HT: Val.has_type (Val.loword (ls (R src))) (mreg_type dst)).
+  assert (HT: Val.has_type (Val.loword (ls @ (R src))) (mreg_type dst)).
   {
     destruct H3. simpl in H5. InvBooleans.
     destruct (mreg_type dst) eqn:T; simpl; auto; inversion H6;
-      destruct (ls (R src)); simpl; auto.
+      destruct (ls @ (R src)); simpl; auto.
   }
   exploit IHmv; eauto. eapply subst_loc_part_satisf_lowlong; eauto.
   destruct H3; InvBooleans. split; eauto using wt_setreg.
   intros [ls' [A B]]. exists ls'; split; auto. eapply star_left; eauto.
   econstructor. simpl; eauto. reflexivity. traceEq.
 + (* highlong *)
-  assert (HT: Val.has_type (Val.hiword (ls (R src))) (mreg_type dst)).
+  assert (HT: Val.has_type (Val.hiword (ls @ (R src))) (mreg_type dst)).
   {
     destruct H3. simpl in H5. InvBooleans.
     destruct (mreg_type dst) eqn:T; simpl; auto; inversion H6;
-      destruct (ls (R src)); simpl; auto.
+      destruct (ls @ (R src)); simpl; auto.
   }
   exploit IHmv; eauto. eapply subst_loc_part_satisf_highlong; eauto.
   destruct H3; InvBooleans. split; eauto using wt_setreg.
@@ -2541,7 +2543,7 @@ Proof.
   assert (F2': eval_addressing tge sp addr (reglist ls3 args2') = Some a2').
     rewrite <- F2. apply eval_addressing_preserved. exact symbols_preserved.
   exploit (eval_offset_addressing tge); eauto. intros F2''.
-  assert (STOREX: exists m2', Mem.storev Mint32 m1' (Val.add a2' (Vint (Int.repr 4))) (ls3 (R src2')) = Some m2' /\ Mem.extends m' m2').
+  assert (STOREX: exists m2', Mem.storev Mint32 m1' (Val.add a2' (Vint (Int.repr 4))) (ls3 @ (R src2')) = Some m2' /\ Mem.extends m' m2').
   { try discriminate;
     (eapply Mem.storev_extends;
      [eexact EXT1 | eexact STORE2 | apply Val.add_lessdef; [eexact G2|eauto] | eauto]). }
@@ -2692,7 +2694,7 @@ Proof.
   split; auto.
   eapply wt_function_wt_bblock; eauto.
   intros [ls1 [A1 [B1 C1]]].
-  assert (Val.lessdef (Vint n) (ls1 (R arg'))).
+  assert (Val.lessdef (Vint n) (ls1 @ (R arg'))).
     rewrite <- H0. eapply add_equation_lessdef with (q := Eq Full arg (R arg')); eauto.
   inv H2.
   econstructor; split.
@@ -2742,8 +2744,8 @@ Proof.
   rewrite H13. apply WTRS.
   generalize (loc_result_caller_save (RTL.fn_sig f)).
   destruct (loc_result (RTL.fn_sig f)); simpl.
-  intros A; rewrite A; auto.
-  intros [A B]; rewrite A, B; auto.
+  intros A; unfold Locmap.get, return_regs; rewrite A; auto.
+  intros [A B]; unfold Locmap.get, return_regs; rewrite A, B; auto.
   apply return_regs_agree_callee_save.
   unfold proj_sig_res. rewrite <- H11; rewrite H13. apply WTRS.
 
